Change class based CavaArrow to an Inductive type named Circuit

cava/arrow-examples/Aes/sbox.v
@@ -34,7 +34,7 @@ Open Scope kind_scope.
 ); *)
 Program Definition aes_sbox
   (sbox_type: SboxImpl)
-  : forall cava: Cava, <<Bit, Vector Bit 8, Unit>> ~> (Vector Bit 8) :=
+  :  <<Bit, Vector Bit 8, Unit>> ~> (Vector Bit 8) :=
   <[\ op_i data_i =>
       let data_o = !(
         match sbox_type with
@@ -82,13 +82,13 @@ Section regression_testing.
   Notation "# x" := (nat_to_bitvec_sized 8 x, tt) (at level 99).
 
   (* Check equal at some random points *)
-  Goal aes_sbox_lut Combinational (false, #0) = aes_sbox_canright Combinational (false, #0).
+  Goal combinational_evaluation' aes_sbox_lut (false, #0) = combinational_evaluation' aes_sbox_canright (false, #0).
+    time vm_compute; auto.
+  Qed.
+  Goal combinational_evaluation' aes_sbox_lut (false, #88) = combinational_evaluation' aes_sbox_canright (false, #88).
     vm_compute; auto.
   Qed.
-  Goal aes_sbox_lut Combinational (false, #88) = aes_sbox_canright Combinational (false, #88).
-    vm_compute; auto.
-  Qed.
-  Goal aes_sbox_lut Combinational (false, #127) = aes_sbox_canright Combinational (false, #127).
+  Goal combinational_evaluation' aes_sbox_lut (false, #127) = combinational_evaluation' aes_sbox_canright (false, #127).
     vm_compute; auto.
   Qed.
 
@@ -122,43 +122,20 @@ Section regression_testing.
     apply H.
   Qed.
 
-  (* TODO(blaxill): works for x < 256 but is slow ... *)
-  Goal forall x, x < 5 -> aes_sbox_lut Combinational (false, #x) = aes_sbox_canright Combinational (false, #x).
+  (* Goal forall x, x < 256 -> combinational_evaluation' aes_sbox_lut (false, #x) = combinational_evaluation' aes_sbox_canright (false, #x).
   Proof.
     apply (reduce_num' _ (fun x =>
-      aes_sbox_lut Combinational (false, # x) =
-      aes_sbox_canright Combinational (false, # x)
+      combinational_evaluation' aes_sbox_lut (false, # x) =
+      combinational_evaluation' aes_sbox_canright (false, # x)
     )).
     Ltac t := apply (reduce_num _ (fun x =>
-      aes_sbox_lut Combinational (false, # x) =
-      aes_sbox_canright Combinational (false, # x)
+      combinational_evaluation' aes_sbox_lut (false, # x) =
+      combinational_evaluation' aes_sbox_canright (false, # x)
     ) _).
     repeat t.
     apply rm_false.
 
     time vm_compute; auto 256.
-  Qed.
-
-  Goal forall x, x < 10 -> aes_sbox_lut Combinational (false, #x) = aes_sbox_canright Combinational (false, #x).
-  Proof.
-    apply (reduce_num' _ (fun x =>
-      aes_sbox_lut Combinational (false, # x) =
-      aes_sbox_canright Combinational (false, # x)
-    )).
-    repeat t.
-    apply rm_false.
-    repeat match goal with
-    | |- context[aes_sbox_lut Combinational ?X] =>
-      let x := fresh in set (x:=aes_sbox_lut Combinational X);
-      vm_compute in x;
-      simpl in x
-    end.
-    unfold aes_sbox_canright;
-    repeat rewrite expression_evaluation_is_arrow_evaluation;
-    set (Z:=interp_combinational _);
-    cbv [interp_combinational] in Z;
-    revert Z;
-    time vm_compute; auto 256.
-  Qed.
+  Qed. *)
 
 End regression_testing.
