cava/arrow-examples/ArrowExtraction.v
@@ -23,18 +23,8 @@ From Coq Require Import extraction.ExtrHaskellNatInteger.
 Extraction Language Haskell.
 
 Require Import Combinators.
-Require Import SyntaxExamples.
-Require Import Mux2_1.
-Require Import UnsignedAdder.
-
-Require Import ArrowAdderTutorial.
 
 Extraction Library Combinators.
-Extraction Library SyntaxExamples.
-Extraction Library Mux2_1.
-Extraction Library UnsignedAdder.
-
-Extraction Library ArrowAdderTutorial.
 
 From Cava Require Import Arrow.ArrowExport.
 (* From Cava Require Import Cava.pkg. *)
@@ -47,3 +37,6 @@ Require Import Aes.sbox_canright_pkg.
 Extraction Library sbox_canright_pkg.
 Require Import Aes.sbox_canright.
 Extraction Library sbox_canright.
+
+Require Import Aes.unrolled_cipher.
+Extraction Library unrolled_cipher.
